FunProg simplification

FunProg.v
@@ -55,17 +55,52 @@ Qed.
 Inductive wlpA [A : DTuple.p] (i : instr A) (post : DTuple.arrow A (fun _ => Prop)) : Prop :=
   wlpA_I (P : wlp i (DTuple.to_fun post)).
 
+Lemma wlpA_eqv [pre A i0 i1 post]
+  (E : @eqv A i0 i1)
+  (C : pre -> wlpA i1 post)
+  (P : pre) : wlpA i0 post.
+Proof.
+  constructor.
+  apply E, C, P.
+Qed.
+
 
 Section Instr.
   Local Obligation Tactic := cbn; intros; do 3 intro; try solve [intuition auto].
 
   Program Definition Ret [A : DTuple.p] (x : DTuple.t A) : instr A
     := fun post => post x.
+  Global Arguments Ret [_] _%dtuple.
 
   Program Definition Bind [A B : DTuple.p] (f : instr A) (g : DTuple.arrow A (fun _ => instr B)) : instr B
     := fun post => wlp f (fun x => wlp (DTuple.to_fun g x) post).
   Next Obligation.
     apply wlp_monotone; intro; apply wlp_monotone, LE.
+  Qed.
+
+  Global Add Parametric Morphism A B : (@Bind A B)
+    with signature (@eqv A) ==>
+      (Rel.pull (@DTuple.to_fun A (fun _ => instr B))
+        (Morphisms.pointwise_relation (DTuple.t A) (@eqv B))) ==>
+      @eqv B
+    as Bind_morph.
+  Proof.
+    intros f0 f1 Ef g0 g1 Eg post; cbn.
+    etransitivity.
+    apply Ef.
+    apply Spec.wp_morph. apply wlp_monotone.
+    intro; apply Eg.
+  Qed.
+
+  Lemma Bind_assoc [A B C] f g h:
+    eqv (@Bind B C (@Bind A B f g) h)
+        (Bind f (DTuple.of_fun (fun x => Bind (DTuple.to_fun g x) h))).
+  Proof.
+    intro post; cbn.
+    apply Spec.wp_morph. apply wlp_monotone.
+    intro x.
+    rewrite DTuple.to_of_fun.
+    reflexivity.
   Qed.
 
   Program Definition Call [A : DTuple.p] (s : Spec.t A) : instr A
@@ -75,10 +110,12 @@ Section Instr.
     := fun post => P /\ post DTuple.tt.
 End Instr.
 
-Inductive wlp_formula [A : DTuple.p] (i : instr A) (f : forall post : DTuple.t A -> Prop, Prop) : Prop :=
-  wlp_formulaI (F : forall post, f post -> wlp i post).
+(* WLP formula *)
 
-Section WLP_Formula.
+Section WLP_Formula. 
+  Inductive wlp_formula [A : DTuple.p] (i : instr A) (f : forall post : DTuple.t A -> Prop, Prop) : Prop :=
+    wlp_formulaI (F : forall post, f post -> wlp i post).
+
   Lemma wlp_formulaE [A i f post] (H : @wlp_formula A i f) (F : f post): wlp i post.
   Proof.
     case H; auto.
@@ -173,9 +210,9 @@ Ltac build_wlp_formula_ dmatch :=
   | |- wlp_formula (match ?x with _ => _ end) _ =>
       lazymatch dmatch with
       | true =>
-          tryif (try (case x; [ (* one case *) ]; fail 1))
-          then build_wlp_formula_branch build x
-          else build_wlp_formula_dlet   build x
+          tryif Tac.is_single_case x
+          then build_wlp_formula_dlet   build x
+          else build_wlp_formula_branch build x
       | false =>
           build_wlp_formula_match build x
       end
@@ -199,3 +236,116 @@ Ltac by_wlp_ dmatch :=
   [ build_wlp_formula_ dmatch | cbn].
 
 Ltac by_wlp := by_wlp_ true.
+
+(* Program simplification *)
+
+Section SimplCont.
+  Inductive k_opt (A : DTuple.p) : forall B : DTuple.p, Type :=
+    | KNone : k_opt A A
+    | KSome [B : DTuple.p] (k : DTuple.arrow A (fun _ => instr B)) : k_opt A B.
+  Global Arguments KNone {_}.
+  Global Arguments KSome [_ _].
+
+  Definition k_apply [A B] (i : instr A) (k : k_opt A B) : instr B :=
+    match k with
+    | KNone   => i
+    | KSome k => Bind i k
+    end.
+
+  Local Add Parametric Morphism A B : (@k_apply A B)
+    with signature (@eqv A) ==> (@eq (k_opt A B)) ==> (@eqv B)
+    as k_apply_morh.
+  Proof.
+    intros i0 i1 E [|k]; cbn; rewrite E; reflexivity.
+  Qed.
+
+  Inductive simpl_cont [A B] (i : instr A) (k : k_opt A B) (r : instr B) : Prop :=
+    simpl_contI (E : eqv r (k_apply i k)).
+
+  Lemma eqv_by_simpl_cont [A i0 i1]
+    (S : @simpl_cont A A i0 KNone i1):
+    eqv i0 i1.
+  Proof.
+    symmetry; apply S.
+  Qed.
+
+  Lemma simpl_cont_morph [A B i0 i1] k
+    (E : eqv i0 i1):
+    @simpl_cont A B i0 k (k_apply i1 k).
+  Proof.
+    constructor.
+    rewrite E.
+    reflexivity.
+  Qed.
+
+  Lemma simpl_cont_def [A B] i k:
+    @simpl_cont A B i k (k_apply i k).
+  Proof.
+    constructor; reflexivity.
+  Qed.
+
+  Lemma simpl_cont_Ret [A B] x k:
+    @simpl_cont A B (Ret x) (KSome k) (DTuple.to_fun k x).
+  Proof.
+    constructor; intro; reflexivity.
+  Qed.
+
+  Lemma simpl_cont_Bind [A B C f0 f1 g0 g1 k]
+    (Eg : DTuple.arrow A (fun x =>
+            @simpl_cont B C (DTuple.to_fun g0 x) k (DTuple.to_fun g1 x)))
+    (Ef : @simpl_cont A C f0 (KSome g1) f1):
+    @simpl_cont B C (Bind f0 g0) k f1.
+  Proof.
+    constructor.
+    etransitivity. apply Ef.
+    cbn.
+    etransitivity. apply Bind_morph. reflexivity.
+    { intro x. etransitivity. apply (DTuple.to_fun Eg x).
+      apply R_refl. reflexivity.
+      symmetry. exact (DTuple.to_of_fun _ x). }
+    clear.
+    case k as [|k]; cbn.
+    - apply Bind_morph. reflexivity.
+      intro; rewrite DTuple.to_of_fun. reflexivity.
+    - symmetry; apply Bind_assoc.
+  Qed.
+End SimplCont.
+
+Ltac build_simpl_cont :=
+  let rec build _ :=
+    cbn;
+    lazymatch goal with
+    | |- simpl_cont (Ret _) (KSome _) _ =>
+        refine (simpl_cont_Ret _ _)
+    | |- simpl_cont (Ret _) KNone _ =>
+        refine (simpl_cont_def _ _)
+    | |- simpl_cont (Bind _ _) _ _ =>
+        refine (simpl_cont_Bind _ _);
+        [ cbn; repeat intro; build tt
+        | build tt]
+    | |- simpl_cont (Call _) _ _ =>
+        refine (simpl_cont_def _ _)
+    | |- simpl_cont (Assert _) _ _ =>
+        refine (simpl_cont_def _ _)
+    | |- simpl_cont (match ?x with _ => _ end) _ ?r =>
+        tryif Tac.is_single_case x
+        then (
+          Tac.build_term r ltac:(fun tt => destruct x; shelve);
+          destruct x; build tt
+        ) else (
+          refine (simpl_cont_morph _ _);
+          match goal with |- eqv _ ?r =>
+          Tac.build_term r ltac:(fun tt => destruct x; shelve)
+          end;
+          destruct x; refine (eqv_by_simpl_cont _); build tt
+        )
+    | |- ?g => fail "build_simpl_cont" g
+    end
+  in build tt.
+
+Ltac simpl_prog :=
+  refine (wlpA_eqv _ _);
+  [ refine (eqv_by_simpl_cont _);
+    build_simpl_cont
+  | cbn ].
+  
